# baseURI: https://linked.data.gov.au/def/fsdf
# imports: http://www.w3.org/2004/02/skos/core
# imports: http://www.w3.org/ns/dcat
# imports: http://www.w3.org/ns/prov-o
# imports: https://linked.data.gov.au/def/loci

@prefix : <https://linked.data.gov.au/def/fsdf#> .
@prefix dbo: <http://dbpedia.org/ontology/> .
@prefix dct: <http://purl.org/dc/terms/> .
@prefix owl: <http://www.w3.org/2002/07/owl#> .
@prefix prov: <http://www.w3.org/ns/prov#> .
@prefix rdf: <http://www.w3.org/1999/02/22-rdf-syntax-ns#> .
@prefix rdfs: <http://www.w3.org/2000/01/rdf-schema#> .
@prefix sdo: <http://schema.org/> .
@prefix skos: <http://www.w3.org/2004/02/skos/core#> .
@prefix vann: <http://purl.org/vocab/vann/> .
@prefix xsd: <http://www.w3.org/2001/XMLSchema#> .

dct:hasPart
  a owl:ObjectProperty ;
.
owl:sameAs
  a owl:ObjectProperty ;
.
<https://link.fsdf.org.au/fsdf-dataset/australian-statistical-geographical-standard-boundaries>
  a owl:NamedIndividual ;
.
<https://link.fsdf.org.au/fsdf-dataset/catchment-boundaries>
  a owl:NamedIndividual ;
.
<https://link.fsdf.org.au/fsdf-dataset/geocoded-national-address-file>
  a owl:NamedIndividual ;
.
<https://linked.data.gov.au/dataset/asgs>
  a owl:NamedIndividual ;
  a :Dataset ;
  dct:hasPart <https://linked.data.gov.au/def/asgs#MeshBlock> ;
  dct:hasPart <https://linked.data.gov.au/def/asgs#State> ;
  rdfs:label "Australian Statistical Geographical Standard Boundaries" ;
  owl:sameAs <https://link.fsdf.org.au/fsdf-dataset/australian-statistical-geographical-standard-boundaries> ;
.
<https://linked.data.gov.au/dataset/geofabric-catchments>
  a owl:NamedIndividual ;
  a :Dataset ;
  dct:hasPart <https://linked.data.gov.au/def/geofabric#Catchment> ;
  dct:hasPart <https://linked.data.gov.au/def/geofabric#Waterbody> ;
  rdfs:label "Catchment Boundaries" ;
  owl:sameAs <https://link.fsdf.org.au/fsdf-dataset/catchment-boundaries> ;
.
<https://linked.data.gov.au/dataset/gnaf>
  a owl:NamedIndividual ;
  a :Dataset ;
  dct:hasPart <https://linked.data.gov.au/def/gnaf#Address> ;
  dct:hasPart <https://linked.data.gov.au/def/gnaf#GeocodedPoint> ;
  dct:hasPart <https://linked.data.gov.au/def/gnaf#Locality> ;
  dct:hasPart <https://linked.data.gov.au/def/gnaf#MeshBlockMatch> ;
  dct:hasPart <https://linked.data.gov.au/def/gnaf#StreetLocality> ;
  rdfs:label "Geocoded National Address File" ;
  owl:sameAs <https://link.fsdf.org.au/fsdf-dataset/geocoded-national-address-file> ;
.
<https://linked.data.gov.au/dataset/png>
  a owl:NamedIndividual ;
  a :Dataset ;
  rdfs:label "National Gazeteer of Australia" ;
  owl:sameAs <https://linked.data.gov.au/def/png#Place> ;
.
<https://linked.data.gov.au/def/asgs#MeshBlock>
  a owl:NamedIndividual ;
.
<https://linked.data.gov.au/def/asgs#State>
  a owl:NamedIndividual ;
.
<https://linked.data.gov.au/def/fsdf>
  a owl:Ontology ;
  dct:created "2018-03-07"^^xsd:date ;
  dct:creator <http://orcid.org/0000-0002-8742-7730> ;
  dct:creator <https://linked.data.gov.au/org/ga> ;
  dct:modified "2021-04-21" ;
  dct:publisher <https://linked.data.gov.au/org/anzlic> ;
  vann:preferredNamespacePrefix "fsdf" ;
  rdfs:label "FSDF ontology" ;
  owl:imports <http://www.w3.org/2004/02/skos/core> ;
  owl:imports <http://www.w3.org/ns/dcat> ;
  owl:imports <http://www.w3.org/ns/prov-o> ;
  owl:imports <https://linked.data.gov.au/def/loci> ;
  owl:versionIRI <https://linked.data.gov.au/def/fsdf/1.1> ;
  owl:versionInfo "1.0"@en ;
  owl:versionInfo "This 1.0 is an early version of the ontology but is a great departure from the 0.5 version that was published in 2018. This version concentrates on defining the FSDF concepts, not listing all of the FSDF datasets which are listed in a separate data graph within the overall FSDF Knolwedge Graph"@en ;
  skos:definition "An ontology describing the Calsses of concepts relevant to the [ANZLIC - The Spatial  Information Council](https://www.anzlic.gov.au)'s' Foundation Spatial Data Framework (FSDF) project which is \"a common reference for the assembly and maintenance of Australian and New Zealand foundation level spatial data\""@en ;
.
:Agency
  a owl:Class ;
  rdfs:subClassOf prov:Agent ;
  skos:definition "An FSDF Agency is a Government Organisation that is involved with the FSDF Programme"@en ;
  skos:prefLabel "Agnecy"@en ;
.
:Dataset
  a owl:Class ;
  rdfs:subClassOf <https://linked.data.gov.au/def/loci#Dataset> ;
  skos:definition "An FSDF Dataset is a Loc-I Dataset, that is a dataset of spatial data following the Location Index (Loc-I) protocols. An FDSF Dataset has additional requirements on it for its use within the FSDF Programme, for example, the dataset must be classified according to the FSDF Themes vocabulary and must have various agents (organisations) of relevance to the dataset, such as crator and owner, recorded."@en ;
  skos:prefLabel "Dataset"@en ;
.
:Jurisdiction
  a owl:Class ;
  rdfs:label "Jurisdiction"@en ;
  rdfs:subClassOf prov:Agent ;
  owl:disjointWith :Agency ;
  skos:definition "A Jurisdiction is a Government Organization that has authority within a domain. The specific domains considered by the FSDF Programme are the Australian Commonwealth (Federal), Australian States and Territories and the Commercial sector."@en ;
.
:Mandate
  a owl:Class ;
  rdfs:subClassOf <http://www.w3.org/ns/dcat#Resource> ;
  rdfs:subClassOf prov:Entity ;
  rdfs:subClassOf [
      a owl:Restriction ;
      owl:cardinality "1"^^xsd:nonNegativeInteger ;
      owl:onProperty :responsibleAuthority ;
    ] ;
  skos:definition "An FSDF Mandate is an Australian Commonwealth or State & Territory legislation thatassigns responsibility for FSDF data or operations to an FSDF Agency. An FSDF Mandate is represented as a specialised form of DCAT Resource which ensures that a DCAT-style catalogue of instances of FSDF Mandates can be made."@en ;
  skos:prefLabel "Mandate"@en ;
.
:Theme
  a owl:Class ;
  rdfs:subClassOf skos:Concept ;
  skos:definition "An FSDF Theme is a SKOS Concept, that is a taxonomy classification class of object, used by the FSDF Programme to organise FSDF Datasets"@en ;
  skos:prefLabel "Theme"@en ;
.
:affectsAgency
  a owl:ObjectProperty ;
  rdfs:domain :Mandate ;
  rdfs:range :Agency ;
  skos:definition "A Agency that is subject to the instructions of this Mandate"@en ;
  skos:prefLabel "affects Agency"@en ;
.
:responsibleAuthority
  a owl:ObjectProperty ;
  rdfs:domain :Mandate ;
  rdfs:range [
      a owl:Class ;
      owl:unionOf (
          :Agency
          :Jurisdiction
        ) ;
    ] ;
  skos:prefLabel "responsible authority" ;
.
<https://linked.data.gov.au/def/geofabric#Catchment>
  a owl:NamedIndividual ;
.
<https://linked.data.gov.au/def/geofabric#Waterbody>
  a owl:NamedIndividual ;
.
<https://linked.data.gov.au/def/gnaf#Address>
  a owl:NamedIndividual ;
.
<https://linked.data.gov.au/def/gnaf#GeocodedPoint>
  a owl:NamedIndividual ;
.
<https://linked.data.gov.au/def/gnaf#Locality>
  a owl:NamedIndividual ;
.
<https://linked.data.gov.au/def/gnaf#MeshBlockMatch>
  a owl:NamedIndividual ;
.
<https://linked.data.gov.au/def/gnaf#StreetLocality>
  a owl:NamedIndividual ;
.
<https://linked.data.gov.au/def/png#Place>
  a owl:NamedIndividual ;
.
