# baseURI: https://linked.data.gov.au/def/fsdf
# imports: https://linked.data.gov.au/def/fsdf/common
# prefix: fsdf

@prefix fsdf: <https://linked.data.gov.au/def/fsdf/> .
@prefix asgs: <https://linked.data.gov.au/def/asgs#> .
@prefix dcat: <http://www.w3.org/ns/dcat#> .
@prefix dcterms: <http://purl.org/dc/terms/> .
@prefix geo: <http://www.opengis.net/ont/geosparql#> .
@prefix jurisdictions: <https://linked.data.gov.au/dataset/fsdf/jurisdictions/> .
@prefix ont: <https://linked.data.gov.au/def/fsdf> .
@prefix owl: <http://www.w3.org/2002/07/owl#> .
@prefix prov: <http://www.w3.org/ns/prov#> .
@prefix rdf: <http://www.w3.org/1999/02/22-rdf-syntax-ns#> .
@prefix rdfs: <http://www.w3.org/2000/01/rdf-schema#> .
@prefix sdo: <https://schema.org/> .
@prefix skos: <http://www.w3.org/2004/02/skos/core#> .
@prefix sosa: <http://www.w3.org/ns/sosa/> .
@prefix ssn: <http://www.w3.org/ns/ssn/> .
@prefix themes: <https://linked.data.gov.au/def/fsdf/themes/> .
@prefix time: <http://www.w3.org/2006/time#> .
@prefix vann: <http://purl.org/vocab/vann/> .
@prefix xsd: <http://www.w3.org/2001/XMLSchema#> .


ont:
  a owl:Ontology ;
  dcterms:created "2018-03-07"^^xsd:date ;
  dcterms:creator <https://linked.data.gov.au/org/surround> ;
  dcterms:modified "2021-06-10"^^xsd:date ;
  dcterms:publisher <https://linked.data.gov.au/org/anzlic> ;
  dcterms:license <http://purl.org/NET/rdflicense/cc-by4.0> ;
  dcterms:rights "(c) Australian Government (ICSM), 2021" ;  
  vann:preferredNamespacePrefix "fsdf" ;
  skos:prefLabel "FSDF ontology"@en ;
  owl:imports <https://linked.data.gov.au/def/fsdf/common> ;
  owl:versionIRI <https://linked.data.gov.au/def/fsdf/1.1> ;
  owl:versionInfo "This 1.0 is an early version of the ontology but is a great departure from the 0.5 version that was published in 2018. This version concentrates on defining the FSDF concepts, not listing all of the FSDF datasets which are listed in a separate data graph within the overall FSDF Knolwedge Graph. This version imports the FSDF common elements ontology" ;
  skos:definition """An ontology describing the concepts relevant to the [ANZLIC - The Spatial  Information Council](https://www.anzlic.gov.au)s' Foundation Spatial Data Framework (FSDF) project which is "a common reference for the assembly and maintenance of Australian and New Zealand foundation level spatial data".
  
This contology contains a number of classes relevant to dataset description, management and provenance, such as `Dataset`, `Mandate` (laws/policies causing the generation of datasets), `Agency` (government bodies that own and create datasets) and `Jurisdition` (government bodies that authority within a domain). Additionally, properties that link these classes, such as `affectsAgency` (linking a `Mandate` to an `Agency`).

It also contains taxonomies (vocabularies) used to categorise datasets and sub-dataset elements. The main taxonomy is the "FSDF Themes" and there are many specialised sub-taxonomies for elements within it, such as "FSDF Themes - Physcial Infrastructure".

Also provided here are common properties for FSDF datasets and their contents, such as `hasGroundRelation` (relates an infrastructure Feature to the earth's surface) as well as taxonomies for many of these proerties' values."""@en ;  
  sdo:codeRepository "https://github.com/surroundaustralia/fsdf-kg"^^xsd:anyURI ;
.

<https://linked.data.gov.au/org/surround>
  a sdo:Organization ;
  sdo:name "SURROUND Australia Pty Ltd" ;
  sdo:url "https://surround.com"^^xsd:anyURI ;
.

<https://linked.data.gov.au/org/anzlic>
  a sdo:Organization ;
  sdo:name "ANZLIC - the Spatial Information Council" ;
  sdo:url "https://www.anzlic.gov.au"^^xsd:anyURI ;
.

prov:Agent
  a owl:Class ;
  rdfs:subClassOf owl:Thing ;
  skos:definition "An agent is something that bears some form of responsibility for an activity taking place, for the existence of an entity, or for another agent's activity"@en ;
  skos:prefLabel "Agent"@en ;
.
skos:Concept a owl:Class ;
  skos:prefLabel "Concept"@en ;
  rdfs:subClassOf owl:Thing ;
  rdfs:isDefinedBy <http://www.w3.org/2004/02/skos/core> ;
  skos:definition "An idea or notion; a unit of thought"@en ;
.
fsdf:Fuel a owl:Class ;
  skos:prefLabel "Fuel"@en ;
  rdfs:subClassOf skos:Concept ;
  rdfs:isDefinedBy ont: ;
  skos:definition "A type of fuel used by powerstations. May be renewable or non-renewable. All instances of these are contained within the Fuels taxonomy within the FSDF Knowledge Graph"@en ;
.
fsdf:GroundRelation a owl:Class ;
  skos:prefLabel "Ground Relation"@en ;
  rdfs:subClassOf skos:Concept ;
  rdfs:isDefinedBy ont: ;
  skos:definition "The relations of geospatial Feature to the earth's surface. All instances of these are contained within the Ground Relations taxonomy within the FSDF Knowledge Graph"@en ;
.
fsdf:Material a owl:Class ;
  skos:prefLabel "Material"@en ;
  rdfs:subClassOf skos:Concept ;
  rdfs:isDefinedBy ont: ;
  skos:definition "Types of material used to construct buildings and facilities in various FSDF datasets. All instances of these are contained within the Materials taxonomy within the FSDF Knowledge Graph"@en ;
.
fsdf:ObservableProperty a owl:Class ;
  skos:prefLabel "Observable Property"@en ;
  rdfs:subClassOf skos:Concept ;
  rdfs:isDefinedBy ont: ;
  skos:definition "Properties of Features that may be observed. All instances of these are contained within the Observable Properties taxonomy within the FSDF Knowledge Graph"@en ;
.
fsdf:OperationalStatus a owl:Class ;
  skos:prefLabel "Operational Status"@en ;
  rdfs:subClassOf skos:Concept ;
  rdfs:isDefinedBy ont: ;
  skos:definition "The status of the operations of FSDF infrastructure assets (Features). All instances of these are contained within the Operational Statuses taxonomy within the FSDF Knowledge Graph"@en ;
.
fsdf:PhysicalCondition a owl:Class ;
  skos:prefLabel "Physical Condition"@en ;
  rdfs:subClassOf skos:Concept ;
  rdfs:isDefinedBy ont: ;
  skos:definition "The types of physical condition that buildings and facilities are known to be in, in various FSDF datasets. All instances of these are contained within the Physical Conditions taxonomy within the FSDF Knowledge Graph"@en ;
.
fsdf:PSStructures a owl:Class ;
  skos:prefLabel "Power Station Structures"@en ;
  rdfs:subClassOf skos:Concept ;
  rdfs:isDefinedBy ont: ;
  skos:definition "The types of structure that Power Stations might have. All instances of these are contained within the PSStructures taxonomy within the FSDF Knowledge Graph"@en ;
.
fsdf:Theme a owl:Class ;
  skos:prefLabel "FSDF Theme"@en ;
  rdfs:subClassOf skos:Concept ;
  rdfs:isDefinedBy ont: ;
  skos:definition "A skos:Concept taken from the FSDF programme's controlled list of 'Themes'. All instnaces are contained within the FSDF Themes taxonomy, and sub-taxonomies of it, all within the FSDF Knowledge Graph"@en ;
.

sdo:Organization
  a owl:Class ;
  rdfs:subClassOf prov:Agent ;
  skos:definition "An organization such as a government agency, a school, NGO, corporation, club, or even a whole government"@en ;
  skos:prefLabel "Organisation"@en ;
.
fsdf:Agency
  a owl:Class ;
  rdfs:subClassOf sdo:Organization ;
  skos:definition "An FSDF Agency is a Government Organisation that is involved with the FSDF Programme"@en ;
  skos:prefLabel "Agency"@en ;
  skos:example """# example from the FSDF datagraph Agencies
agencies:nntt
  a fsdf:Agency ;
  sdo:name "National Native Title Tribunal"@en ;
.""" ;
.
dcat:Dataset
  a owl:Class ;
  rdfs:isDefinedby <http://www.w3.org/ns/dcat> ;
  rdfs:subClassOf owl:Thing , prov:Entity , dcat:Resource ;
  skos:definition "A collection of data, published or curated by a single agent, and available for access or download in one or more representations"@en ;
  skos:prefLabel "Dataset"@en ;
.
fsdf:Jurisdiction
  a owl:Class ;
  rdfs:subClassOf sdo:Organization ;
  rdfs:subClassOf dcterms:Jurisdiction ;
  owl:disjointWith fsdf:Agency ;
  skos:definition "A Jurisdiction is a Government Organization that has authority within a domain. The specific domains considered by the FSDF Programme are the Australian Commonwealth (Federal), Australian States and Territories and the Commercial sector"@en ;
  skos:prefLabel "Jurisdiction"@en ;  
.
fsdf:Mandate
  a owl:Class ;
  rdfs:subClassOf sdo:Legislation ;
  rdfs:subClassOf [
      a owl:Restriction ;
      owl:cardinality "1"^^xsd:nonNegativeInteger ;
      owl:onProperty fsdf:hasResponsibleAuthority ;
    ] ;
  skos:definition "An FSDF Mandate is an Australian Commonwealth or State & Territory legislation thatassigns responsibility for FSDF data or operations to an FSDF Agency. An FSDF Mandate is represented as a specialised form of DCAT Resource which ensures that a DCAT-style catalogue of instances of FSDF Mandates can be made"@en ;
  skos:prefLabel "Mandate"@en ;
  skos:example """# example from the FSDF datagraph Mandates
# Here the Mandate is a law (an Act) that was enacted by Victoria
# This Act comples the collection of certain natural-resource datasets by DELWP
mandates:clp-1994
  a fsdf:Mandate ;
  dcterms:title "Catchment and Land Protection Act 1994"@en ;
  fsdf:responsibleAuthority jurisdictions:vic ;
  fsdf:affectsAgency agencies:delwp ;
.""" ;
.
geo:FeatureCollection
  a owl:Class ;
  rdfs:isDefinedby <http://www.opengis.net/ont/geosparql> ;
  rdfs:subClassOf owl:Thing , prov:Entity ;
  skos:definition "The class Feature Collection represents any collection of individual Features"@en ;
  skos:prefLabel "Feature Collection"@en ;
.
geo:Feature
  a owl:Class ;
  rdfs:isDefinedby <http://www.opengis.net/ont/geosparql> ;
  rdfs:subClassOf owl:Thing , prov:Entity ;
  skos:definition "This class represents the top-level feature type. This class is equivalent to GFI_Feature defined in ISO 19156, and it is superclass of all feature types"@en ;
  skos:prefLabel "Feature"@en ;
.
fsdf:affectsAgency
  a owl:ObjectProperty ;
  rdfs:domain fsdf:Mandate ;
  rdfs:range fsdf:Agency ;
  skos:definition "A Agency that is subject to the instructions of this Mandate"@en ;
  skos:prefLabel "affects Agency"@en ;
  skos:example """# example from the FSDF datagraph Mandates
# Here a particular Mandate affects a particular Agency
mandates:clp-1994
  fsdf:affectsAgency agencies:delwp ;
.""" ;  
.
fsdf:hasCustodian
  a owl:ObjectProperty ;
  rdfs:domain dcat:Dataset ;
  rdfs:range fsdf:Agency ;
  rdfs:subPropertyOf dcterms:publisher ;
  rdfs:subPropertyOf prov:agent ;
  skos:definition "The Agency that manages this Dataset"@en ;
  skos:prefLabel "has custodian"@en ;
.
fsdf:hasJurisdiction
  a owl:ObjectProperty ;
  rdfs:range fsdf:Jurisdiction ;
  rdfs:subPropertyOf dcterms:publisher ;
  rdfs:subPropertyOf prov:agent ;
  skos:definition "The Jurisdiction responsible for this object"@en ;
  skos:prefLabel "has jurisdiction"@en ;
.

fsdf:hasPrimaryFuel
  a owl:ObjectProperty ;
  rdfs:domain geo:Feature ;
  rdfs:range fsdf:Fuel ;
  skos:prefLabel "Primary Fuel"@en ;
  skos:definition "The primary fuel type used by a generator"@en ;
.

fsdf:hasPrimarySubFuel
  a owl:ObjectProperty ;
  rdfs:domain geo:Feature ;
  rdfs:range fsdf:Fuel ;
  skos:prefLabel "Primary Sub-fuel"@en ;
  skos:definition "The primary sub-fuel type used by a generator"@en ;
.

fsdf:hasGeneratorNumber
  a owl:ObjectProperty ;
  rdfs:domain geo:Feature ;
  rdfs:range xsd:integer ;
  skos:prefLabel "Generator Number"@en ;
  skos:definition "The generator number for electricity generation infrastructure"@en ;
.

fsdf:hasEmbeddedNetworkOperator
  a owl:ObjectProperty ;
  rdfs:domain geo:Feature ;
  rdfs:range rdfs:Literal ;
  skos:prefLabel "Embedded Network Operator"@en ;
  skos:definition "The embedded network operator identifier for electricity generation infrastructure"@en ;
.

fsdf:hasResponsibleAuthority
  a owl:ObjectProperty ;
  rdfs:domain fsdf:Mandate ;
  rdfs:range [
      a owl:Class ;
      skos:prefLabel "Agency and Jurisdiction Union"@en ;
      skos:definition "Union of all Agency and Jurisdiction instances"@en ;
      owl:unionOf (
          fsdf:Agency
          fsdf:Jurisdiction
        ) ;
    ] ;
  skos:definition "The authority responsible for a Mandate"@en ;
  skos:prefLabel "responsible authority"@en ;
.

fsdf:hasOperationalStatus 
  a owl:ObjectProperty ;
  rdfs:domain geo:Feature ;
  rdfs:range fsdf:OperationalStatus ;
  skos:definition "The mode of physical operation of the feature"@en ;
  skos:prefLabel "has operational status"@en ;
.

fsdf:featureDataProvenance
  a owl:ObjectProperty ;
  rdfs:domain geo:Feature ;
  skos:definition "The provenance (source from which, and date) that feature data was received"@en ;
  skos:prefLabel "feature data provenance"@en ;
.

fsdf:hasRelationToGround
  a owl:ObjectProperty ;
  rdfs:domain geo:Feature ;
  rdfs:range fsdf:GroundRelation ;
  skos:definition "The relation of this Feature to the earth's surface"@en ;
  skos:prefLabel "has relation to ground"@en ;
.

fsdf:themeOfFeatureWithProperty
  a owl:ObjectProperty ;
  rdfs:domain fsdf:Theme ;
  rdfs:range sosa:ObservableProperty ;
  skos:definition "A Feature with this theme has this expected Observable Property"@en ;
  skos:prefLabel "theme of feature with property"@en ;
  skos:example """# example from the feature-property-relations datagraph
themes:electrical-infrastructure
  fsdf:themeOfFeatureWithProperty obsp:ratedVoltage ;
.""" ;
.

fsdf:likelyPropertyOfFeatureWithTheme
  a owl:ObjectProperty ;
  owl:inverseOf fsdf:hasExpectedObservableProperty ;
  rdfs:domain sosa:ObservableProperty ;
  rdfs:range fsdf:Theme ;  
  skos:definition "This Observable Property is expected to be of a Feature with this theme"@en ;
  skos:prefLabel "likely property of feature with theme"@en ;
  skos:example """# example from the feature-property-relations datagraph
obsp:ratedVoltage 
  fsdf:likelyPropertyOfFeatureWithTheme themes:electrical-infrastructure ;
.""" ;
.

# from SOSA

sosa:FeatureOfInterest a owl:Class ;
	rdfs:subClassOf owl:Thing ;
	skos:prefLabel "Feature Of Interest"@en ;
	skos:definition "The thing whose property is being estimated or calculated in the course of an Observation to arrive at a Result or whose property is being manipulated by an Actuator, or which is being sampled or transformed in an act of Sampling"@en ;
	rdfs:isDefinedBy sosa: ;
.
sosa:ObservableProperty a owl:Class ;
	rdfs:subClassOf owl:Thing ;
	skos:prefLabel "Observable Property"@en ;
    skos:definition "An observable quality (property, characteristic) of a FeatureOfInterest"@en ;
    skos:example "The height of a tree, the depth of a water body, or the temperature of a surface are examples of observable properties, while the value of a classic car is not (directly) observable but asserted."^^rdf:HTML ;
    rdfs:isDefinedBy sosa: ;
.
sosa:usedProcedure a owl:ObjectProperty ;
    skos:prefLabel "used procedure"@en ;
    skos:definition "A relation to link to a re-usable Procedure used in making an Observation, an Actuation, or a Sample, typically through a Sensor, Actuator or Sampler"@en ;
    rdfs:domain sosa:Actuation ;
    rdfs:domain sosa:Observation ;
    rdfs:domain sosa:Sampling ;
    rdfs:range sosa:Procedure ;
    rdfs:isDefinedBy sosa: ;
.
sosa:hasFeatureOfInterest a owl:ObjectProperty ;
    skos:prefLabel "has feature of interest"@en ;
    skos:definition "A relation between an Observation and the entity whose quality was observed, or between an Actuation and the entity whose property was modified, or between an act of Sampling and the entity that was sampled"@en ;
    skos:example "For example, in an Observation of the weight of a person, the FeatureOfInterest is the person and the property is its weight."^^rdf:HTML ;
    rdfs:domain sosa:Observation ;
    rdfs:domain sosa:Actuation ;
    rdfs:domain sosa:Sampling ;
    rdfs:range sosa:FeatureOfInterest ;
    owl:inverseOf sosa:isFeatureOfInterestOf ;
    rdfs:isDefinedBy sosa: ;
.
sosa:isFeatureOfInterestOf a owl:ObjectProperty ;
    skos:prefLabel "is feature of interest of"@en ;
    skos:definition "A relation between a FeatureOfInterest and an Observation about it, an Actuation acting on it, or an act of Sampling that sampled it"@en ;
    rdfs:domain sosa:FeatureOfInterest ;
    rdfs:domain sosa:Sample ;
    rdfs:range sosa:Observation ;
    rdfs:range sosa:Actuation ;
    rdfs:range sosa:Sampling ;
    owl:inverseOf sosa:hasFeatureOfInterest ;
    rdfs:isDefinedBy sosa: ;
.
sosa:Observation a owl:Class ;
	rdfs:subClassOf owl:Thing ;
    skos:prefLabel "Observation"@en ;
    skos:definition "Act of carrying out an (Observation) Procedure to estimate or calculate a value of a property of a FeatureOfInterest. Links to a Sensor to describe what made the Observation and how; links to an ObservableProperty to describe what the result is an estimate of, and to a FeatureOfInterest to detail what that property was associated with"@en ;
    skos:example "The activity of estimating the intensity of an Earthquake using the Mercalli intensity scale is an Observation as is measuring the moment magnitude, i.e., the energy released by said earthquake."^^rdf:HTML ;
    rdfs:isDefinedBy sosa: ;
.
sosa:observedProperty a owl:ObjectProperty ;
    skos:prefLabel "observed property"@en ;
    skos:definition "Relation linking an Observation to the property that was observed. The ObservableProperty should be a property of the FeatureOfInterest (linked by hasFeatureOfInterest) of this Observation"@en ;
    rdfs:domain sosa:Observation ;
    rdfs:range sosa:ObservableProperty ;
    rdfs:isDefinedBy sosa: ;
.
sosa:Result a owl:Class ;
    skos:prefLabel "Result"@en ;
    skos:definition "The Result of an Observation, Actuation, or act of Sampling. To store an observation's simple result value one can use the hasSimpleResult property"@en ;
    skos:example "The value 20 as the height of a certain tree together with the unit, e.g., Meter."^^rdf:HTML ;
    rdfs:isDefinedBy sosa: ;
    rdfs:subClassOf sosa:Sample ;
.
sosa:hasResult a owl:ObjectProperty ;
    skos:prefLabel "has result"@en ;
    skos:definition "Relation linking an Observation or Actuation or act of Sampling and a Result or Sample"@en ;
    rdfs:domain sosa:Actuation ;
    rdfs:domain sosa:Observation ;
    rdfs:domain sosa:Sampling ;
    rdfs:range sosa:Result ;
    rdfs:range sosa:Sample ;
    owl:inverseOf sosa:isResultOf ;
    rdfs:isDefinedBy sosa: ;
.
sosa:isResultOf a owl:ObjectProperty ;
    skos:prefLabel "is result of"@en ;
    skos:definition "Relation linking a Result to the Observation or Actuation or act of Sampling that created or caused it"@en ;
    rdfs:domain sosa:Result ;
    rdfs:domain sosa:Sample ;
    rdfs:range sosa:Actuation ;
    rdfs:range sosa:Observation ;
    rdfs:range sosa:Sampling ;
    owl:inverseOf sosa:hasResult ;
    rdfs:isDefinedBy sosa: ;
.
sosa:hasSimpleResult a owl:DatatypeProperty ;
    skos:prefLabel "has simple result"@en ;
    skos:definition "The simple value of an Observation or Actuation or act of Sampling"@en ;
    skos:example "For instance, the values 23 or true."^^rdf:HTML ;
    rdfs:domain sosa:Actuation ;
    rdfs:domain sosa:Observation ;
    rdfs:domain sosa:Sampling ;
    rdfs:isDefinedBy sosa: ;
.
sosa:resultTime a owl:DatatypeProperty ;
    skos:prefLabel "result time"@en ;
    skos:definition "The result time is the instant of time when the Observation, Actuation or Sampling activity was completed"@en ;
    rdfs:domain sosa:Actuation ;
    rdfs:domain sosa:Observation ;
    rdfs:domain sosa:Sampling ;
    rdfs:range xsd:dateTime ;
    rdfs:isDefinedBy sosa: ;
.
sosa:phenomenonTime a owl:ObjectProperty ;
    skos:prefLabel "phenomenon time"@en ;
    skos:definition "The time that the Result of an Observation, Actuation or Sampling applies to the FeatureOfInterest. Not necessarily the same as the resultTime. May be an Interval or an Instant, or some other compound TemporalEntity"@en ;
    rdfs:domain sosa:Actuation ;
    rdfs:domain sosa:Observation ;
    rdfs:domain sosa:Sampling ;
    rdfs:range time:TemporalEntity ;
    rdfs:isDefinedBy sosa: ;
.

# from SSN-ext

sosa:ObservationCollection
    a owl:Class ;
    rdfs:subClassOf owl:Thing ;
    skos:definition "Collection of observations, typically with one or more property shared by all of its members"@en ;
    skos:prefLabel "Collection of observations"@en ;
    rdfs:subClassOf sosa:Observation ;
    rdfs:subClassOf [
        a owl:Restriction ;
        owl:allValuesFrom sosa:FeatureOfInterest ;
        owl:onProperty sosa:hasFeatureOfInterest ;
    ] ;
    rdfs:subClassOf [
        a owl:Restriction ;
        owl:allValuesFrom sosa:FeatureOfInterest ;
        owl:onProperty sosa:hasUltimateFeatureOfInterest ;
    ] ;
    rdfs:subClassOf [
        a owl:Restriction ;
        owl:allValuesFrom sosa:ObservableProperty ;
        owl:onProperty sosa:observedProperty ;
    ] ;
    rdfs:subClassOf [
        a owl:Restriction ;
        owl:allValuesFrom sosa:Procedure ;
        owl:onProperty sosa:usedProcedure ;
    ] ;
    rdfs:subClassOf [
        a owl:Restriction ;
        owl:allValuesFrom sosa:Sensor ;
        owl:onProperty sosa:madeBySensor ;
    ] ;
    rdfs:subClassOf [
        a owl:Restriction ;
        owl:allValuesFrom ssn:Stimulus ;
        owl:onProperty ssn:wasOriginatedBy ;
    ] ;
    rdfs:subClassOf [
        a owl:Restriction ;
        owl:maxCardinality "1"^^xsd:nonNegativeInteger ;
        owl:onProperty sosa:hasFeatureOfInterest ;
    ] ;
    rdfs:subClassOf [
        a owl:Restriction ;
        owl:maxCardinality "1"^^xsd:nonNegativeInteger ;
        owl:onProperty sosa:hasUltimateFeatureOfInterest ;
    ] ;
    rdfs:subClassOf [
        a owl:Restriction ;
        owl:maxCardinality "1"^^xsd:nonNegativeInteger ;
        owl:onProperty sosa:madeBySensor ;
    ] ;
    rdfs:subClassOf [
        a owl:Restriction ;
        owl:maxCardinality "1"^^xsd:nonNegativeInteger ;
        owl:onProperty sosa:observedProperty ;
    ] ;
    rdfs:subClassOf [
        a owl:Restriction ;
        owl:maxCardinality "1"^^xsd:nonNegativeInteger ;
        owl:onProperty sosa:phenomenonTime ;
    ] ;
    rdfs:subClassOf [
        a owl:Restriction ;
        owl:maxCardinality "1"^^xsd:nonNegativeInteger ;
        owl:onProperty sosa:resultTime ;
    ] ;
    rdfs:subClassOf [
        a owl:Restriction ;
        owl:maxCardinality "1"^^xsd:nonNegativeInteger ;
        owl:onProperty sosa:usedProcedure ;
    ] ;
    rdfs:subClassOf [
        a owl:Restriction ;
        owl:minCardinality "1"^^xsd:nonNegativeInteger ;
        owl:onProperty sosa:hasMember ;
    ] ;
.

sosa:hasFeatureOfInterest
    rdfs:domain sosa:ObservationCollection ;
.
sosa:hasMember
    a owl:ObjectProperty ;
    rdfs:domain sosa:ObservationCollection ;
    rdfs:range sosa:Observation ;
    skos:definition "Link to a member within a collection of (observations) or (collections of observations) that share the same value for one or more of the characteristic properties"@en ;
    rdfs:domain sosa:ObservationCollection ;
    skos:prefLabel "has member"@en ;
    rdfs:range sosa:Observation ;
    rdfs:subPropertyOf rdfs:member ;
.
sosa:observedProperty
    rdfs:domain sosa:ObservationCollection ;
.
sosa:phenomenonTime
    rdfs:domain sosa:ObservationCollection ;
.
sosa:resultTime
    rdfs:domain sosa:ObservationCollection ;
.
sosa:usedProcedure
    rdfs:domain sosa:ObservationCollection ;
.
	