# baseURI: https://linked.data.gov.au/def/fsdf/observable-properties
# prefix: obsp

@prefix cs: <https://linked.data.gov.au/def/fsdf/observable-properties> .
@prefix dcterms: <http://purl.org/dc/terms/> .
@prefix owl: <http://www.w3.org/2002/07/owl#> .
@prefix rdf: <http://www.w3.org/1999/02/22-rdf-syntax-ns#> .
@prefix rdfs: <http://www.w3.org/2000/01/rdf-schema#> .
@prefix skos: <http://www.w3.org/2004/02/skos/core#> .
@prefix obsp: <https://linked.data.gov.au/def/fsdf/observable-properties/> .
@prefix xsd: <http://www.w3.org/2001/XMLSchema#> .


cs: 
    a owl:Ontology , skos:ConceptScheme ;
    skos:prefLabel "FSDF Observable Properties" ;
    dcterms:creator <https://linked.data.gov.au/org/ga> ;
    dcterms:publisher <https://linked.data.gov.au/org/icsm> ;
    dcterms:created "2021-05-13"^^xsd:date ;
    dcterms:modified "2021-05-13"^^xsd:date ;
    dcterms:provenance "Created for the Loc-I DR Project" ;
    skos:definition "This vocabulary lists physical properties of Features that may be observed to gain measurements of capacities of the Feature" ;
    owl:versionInfo "1.0"^^xsd:string ;
    skos:hasTopConcept
    	obsp:ratedVoltage ,
        obsp:population ,
        obsp:populationChange ;
.

obsp:ratedVoltage
    a skos:Concept ;
    skos:prefLabel "Rated Voltage"@en ;
    skos:definition "The voltage that the Feature is rated to carry or operate at"@en ;
    rdfs:isDefinedBy cs: ;
    skos:inScheme cs: ;
    skos:topConceptOf cs: ;
.

obsp:population
    a skos:Concept ;
    skos:prefLabel "Population"@en ;
    skos:definition "The total count of people for a given Feature"@en ;
    rdfs:isDefinedBy cs: ;
    skos:inScheme cs: ;
    skos:topConceptOf cs: ;
.

obsp:populationChange
    a skos:Concept ;
    skos:prefLabel "Population Change"@en ;
    skos:definition "The change in population for a given Feature and a given teporal interval"@en ;
    rdfs:isDefinedBy cs: ;
    skos:inScheme cs: ;
    skos:topConceptOf cs: ;
.

